explicit map attempt, non target done

theories/Logic/inverse_neg.v
@@ -8,6 +8,8 @@ From Cyclic_PA.Logic Require Import proof_trees.
 From Cyclic_PA.Logic Require Import substitute.
 From Cyclic_PA.Logic Require Import PA_cyclic.
 
+Require Import Coq.Arith.Wf_nat.
+
 Require Import List.
 Import ListNotations.
 
@@ -151,7 +153,7 @@ match P, S with
       (dub_neg_sub_formula C E SC)
       A n d1 d2 alpha1 alpha2
       (dub_neg_sub_ptree_fit P1 E (lor_ind SC (non_target A)))
-      P2
+      (dub_neg_sub_ptree_fit P2 E (lor_ind SC (non_target A)))
 
 | cut_ca C A d1 d2 alpha1 alpha2 P1 P2, _ =>
     cut_ca
@@ -176,10 +178,63 @@ match P, S with
 | _, _ => P
 end.
 
+Fixpoint dub_neg_node_fit (P : ptree) (S : subst_ind) : list subst_ind :=
+match P, S with
+| deg_up d P', _ => dub_neg_node_fit P' S
+
+| ord_up alpha P', _ => dub_neg_node_fit P' S
+
+| node A, _ => [S]
+
+| exchange_ab A B d alpha P', (lor_ind S_B S_A) => dub_neg_node_fit P' (lor_ind S_A S_B)
+
+| exchange_cab C A B d alpha P', (lor_ind (lor_ind S_C S_B) S_A) => dub_neg_node_fit P' (lor_ind (lor_ind S_C S_A) S_B)
+
+| exchange_abd A B D d alpha P', (lor_ind (lor_ind S_B S_A) S_D) => dub_neg_node_fit P' (lor_ind (lor_ind S_A S_B) S_D)
+
+| exchange_cabd C A B D d alpha P', (lor_ind (lor_ind (lor_ind S_C S_B) S_A) S_D) => dub_neg_node_fit P' (lor_ind (lor_ind (lor_ind S_C S_A) S_B) S_D)
+
+| contraction_a A d alpha P', _ => dub_neg_node_fit P' (lor_ind S S)
+
+| contraction_ad A D d alpha P', (lor_ind S_A S_D) => dub_neg_node_fit P' (lor_ind (lor_ind S_A S_A) S_D)
+
+| weakening_ad A D d alpha P', (lor_ind S_A S_D) => dub_neg_node_fit P' S_D
+
+| demorgan_ab A B d1 d2 alpha1 alpha2 P1 P2, _ => dub_neg_node_fit P1 (0) ++ dub_neg_node_fit P2 (0)
+
+| demorgan_abd A B D d1 d2 alpha1 alpha2 P1 P2, (lor_ind S_AB S_D) => dub_neg_node_fit P1 (lor_ind (0) S_D) ++ dub_neg_node_fit P2 (lor_ind (0) S_D)
+
+| negation_a A d alpha P', _ => dub_neg_node_fit P' (non_target A)
+
+| negation_ad A D d alpha P', (lor_ind S_A S_D) => dub_neg_node_fit P' (lor_ind (non_target A) S_D)
+
+| quantification_a A n t d alpha P', _ => dub_neg_node_fit P' (0)
+
+| quantification_ad A D n t d alpha P', (lor_ind S_A S_D) => dub_neg_node_fit P' (lor_ind (0) S_D)
+
+| loop_a A n d1 d2 alpha1 alpha2 P1 P2, _ => (snd (split (filter (fun X => if form_eq_dec A (fst X) then false else true) (combine (node_extract P2) (dub_neg_node_fit P2 (non_target A)))))) ++ dub_neg_node_fit P1 (non_target A)
+
+| loop_ca C A n d1 d2 alpha1 alpha2 P1 P2, (lor_ind S_C S_A) => (snd (split (filter (fun X => if form_eq_dec (lor C A) (fst X) then false else true) (combine (node_extract P2) (dub_neg_node_fit P2 (lor_ind S_C (non_target A))))))) ++ dub_neg_node_fit P1 (lor_ind S_C (non_target A))
+
+| cut_ca C A d1 d2 alpha1 alpha2 P1 P2, _ => dub_neg_node_fit P1 (lor_ind S (non_target A)) ++ dub_neg_node_fit P2 (0)
+
+| cut_ad A D d1 d2 alpha1 alpha2 P1 P2, _ => dub_neg_node_fit P1 (non_target A) ++ dub_neg_node_fit P2 (lor_ind (0) S)
+
+| cut_cad C A D d1 d2 alpha1 alpha2 P1 P2, (lor_ind S_C S_D) => dub_neg_node_fit P1 (lor_ind S_C (non_target A)) ++ dub_neg_node_fit P2 (lor_ind (0) S_D)
+
+| _,_ => []
+end.
+
 Definition dub_neg_sub_ptree (P : ptree) (E : formula) (S : subst_ind) : ptree :=
 match subst_ind_fit (ptree_formula P) S with
 | false => P
 | true => dub_neg_sub_ptree_fit P E S
+end.
+
+Definition dub_neg_node (P : ptree) (S : subst_ind) : list subst_ind :=
+match subst_ind_fit (ptree_formula P) S with
+| false => map non_target (node_extract P)
+| true => dub_neg_node_fit P S
 end.
 
 Lemma dub_neg_ptree_formula_true :
@@ -187,6 +242,12 @@ Lemma dub_neg_ptree_formula_true :
         subst_ind_fit (ptree_formula P) S = true ->
             dub_neg_sub_ptree_fit P E S = dub_neg_sub_ptree P E S.
 Proof. intros. unfold dub_neg_sub_ptree. destruct P; rewrite H; auto. Qed.
+
+Lemma dub_neg_node_formula_true :
+    forall (P : ptree) (S : subst_ind),
+        subst_ind_fit (ptree_formula P) S = true ->
+            dub_neg_node_fit P S = dub_neg_node P S.
+Proof. intros. unfold dub_neg_node. rewrite H. reflexivity. Qed.
 
 Lemma dub_neg_axiom_id :
     forall (A E : formula) (S : subst_ind),
@@ -399,6 +460,994 @@ all : unfold ptree_deg; fold ptree_deg;
       try reflexivity.
 Qed.
 
+Definition dub_neg_trans (L : (list (formula * subst_ind))) (E : formula) := map (fun A => dub_neg_sub_formula (fst A) E (snd A)) L.
+
+Lemma combine_eq_len :
+    forall {A B : Type} (L1 L3 : list A) (L2 L4 : list B),
+        length L1 = length L2 ->
+            combine L1 L2 ++ combine L3 L4 = combine (L1 ++ L3) (L2 ++ L4).
+Proof.
+intros A B L1.
+induction L1;
+intros L3 L2 L4 EQ;
+destruct L2.
+- reflexivity.
+- inversion EQ.
+- inversion EQ.
+- repeat rewrite <- app_comm_cons.
+  unfold combine;
+  fold (@combine A A).
+  rewrite <- IHL1.
+  reflexivity.
+  apply eq_add_S, EQ.
+Qed.
+
+Lemma combine_filter_fst :
+    forall {A B : Type} (L1 : list A) (L2 : list B) (f : A -> bool),
+        length L1 = length L2 ->
+            length (filter (fun X => f (fst X)) (combine L1 L2)) = length (filter f L1).
+Proof.
+intros A B L1.
+induction L1;
+intros L2 f EQL;
+destruct L2.
+- reflexivity.
+- inversion EQL.
+- inversion EQL.
+- unfold combine;
+  fold (@combine A B).
+  unfold filter;
+  fold (filter f) (filter (fun (X : A * B) => f (fst X))).
+  unfold fst at 1.
+  case (f a) eqn:T.
+  + unfold length;
+    fold (@length A) (@length (A*B)).
+    rewrite IHL1.
+    reflexivity.
+    apply eq_add_S, EQL.
+  + apply IHL1, eq_add_S, EQL.
+Qed.
+
+Lemma combine_non_target_triv : 
+  forall (L : list formula) (E : formula),
+      dub_neg_trans (combine L (map non_target L)) E = L.
+Proof.
+induction L;
+intros E.
+- reflexivity.
+- unfold map, combine;
+  fold (map non_target) (@combine formula subst_ind).
+  unfold dub_neg_trans in *.
+  unfold map at 1.
+  fold (map (fun A : formula * subst_ind => dub_neg_sub_formula (fst A) E (snd A))).
+  unfold dub_neg_sub_formula at 1.
+  rewrite non_target_sub.
+  rewrite (IHL E).
+  reflexivity.
+Qed.
+
+Lemma non_target_lor :
+    forall {A B : formula},
+        (lor_ind (non_target A) (non_target B)) = (non_target (lor A B)). Proof. reflexivity. Qed.
+
+Lemma eq_app_eq :
+    forall {A : Type} (L1 L2 L3 L4 : list A),
+        L1 = L2 -> L3 = L4 -> L1 ++ L3 = L2 ++ L4.
+Proof.
+intros A L1 L2 L3 L4 EQ1 EQ2.
+rewrite EQ1, EQ2.
+reflexivity.
+Qed.
+
+Lemma snd_split :
+    forall {A B : Type} {L : list (A * B)} {a : A} {b : B},
+        snd (split ((a,b) :: L)) = b :: snd (split L).
+Proof.
+intros A B L a b.
+unfold split at 1.
+fold (split L).
+unfold snd at 1.
+destruct (split L).
+reflexivity.
+Qed.
+    
+Lemma combine_with_filter_split :
+    forall {A B : Type} (f : A -> bool) (L1 : list A) (L2 : list B),
+        length L1 = length L2 ->
+            combine (filter f L1) (snd (split (filter (fun X => f (fst X)) (combine L1 L2)))) = (filter (fun X => f (fst X)) (combine L1 L2)).
+Proof.
+intros A B f.
+induction L1;
+intros L2 EQL;
+destruct L2.
+- reflexivity.
+- inversion EQL.
+- inversion EQL.
+- unfold length in EQL;
+  fold (@length A) (@length B) in EQL.
+  unfold combine;
+  fold (@combine A B).
+  unfold filter;
+  fold (@filter A f) (@filter (A * B) (fun X => f (fst X))).
+  unfold fst at 1 4.
+  case (f a) eqn:Val.
+  + rewrite snd_split.
+    unfold combine at 1.
+    fold (@combine A B).
+    rewrite IHL1.
+    reflexivity.
+    apply (eq_add_S _ _ EQL).
+  + rewrite IHL1.
+    reflexivity.
+    apply (eq_add_S _ _ EQL).
+Qed.
+
+Lemma filter_fst_non_target : 
+    forall {A B : Type} (f : A -> bool) (m : A -> B) (L : list A),
+        (snd (split (filter (fun X => f (fst X)) (combine L (map m L))))) = map m (filter (fun X => f X) L).
+Proof.
+intros A B f m L.
+induction L.
+- reflexivity.
+- unfold combine, map.
+  fold (map m) (combine L (map m L)).
+  unfold filter;
+  fold (filter f) (filter (fun (X : A * B) => (f (fst X)))).
+  unfold fst at 1.
+  case (f a) eqn:T;
+  try rewrite snd_split;
+  rewrite IHL;
+  reflexivity.
+Qed.
+
+Lemma dub_neg_node_non_target :
+    forall (P : ptree),
+        struct_valid P ->
+            dub_neg_node P (non_target (ptree_formula P)) = map non_target (node_extract P).
+Proof.
+intros P.
+induction P;
+intros PSV;
+unfold dub_neg_node, node_extract, dub_neg_node_fit;
+rewrite non_target_fit;
+fold node_extract dub_neg_node_fit.
+
+1 : destruct PSV. (*node*)
+2 : destruct PSV as [PSV DU]. (*deg up*)
+3 : destruct PSV as [[PSV OU] NO]. (*ord up*)
+
+4-13 : destruct PSV as [[[PF PSV] PD] PO]. (*single hyp*)
+14 : destruct PSV as [[[[PF PSV] PD] PO] CPF]. (*weakening*)
+
+15-19 : destruct PSV as [[[[[[[P1F P1SV] P1D] P1O] P2F] P2SV] P2D] P2O]. (*double hyp*)
+20-21 : destruct PSV as [[[[[[[[P1F P1SV] P1D] P1O] P2F] P2SV] P2D] P2O] INA]. (*loop*)
+
+1 : reflexivity.
+
+
+all : unfold ptree_formula;
+      fold ptree_formula;
+      unfold non_target;
+      fold non_target;
+      repeat rewrite dub_neg_node_formula_true;
+      repeat rewrite non_target_lor.
+
+all : try rewrite <- (IHP PSV);
+      try rewrite map_app;
+      try rewrite <- (IHP1 P1SV);
+      try rewrite <- (IHP2 P2SV);
+      try rewrite PF;
+      try rewrite P1F;
+      try rewrite P2F;
+      unfold subst_ind_fit;
+      fold subst_ind_fit;
+      unfold non_target;
+      fold non_target;
+      repeat rewrite non_target_fit;
+      repeat rewrite non_target_sub_fit;
+      try reflexivity.
+
+all : rewrite <- non_target_term_sub;
+      rewrite (non_target_term_sub a n (succ (var n))) at 1;
+      try rewrite non_target_lor;
+      rewrite <- P2F;
+      rewrite (IHP2 P2SV);
+      try rewrite (filter_fst_non_target (fun X => if form_eq_dec a X then false else true));
+      try rewrite (filter_fst_non_target (fun X => if form_eq_dec (lor c a) X then false else true));
+      rewrite <- remove_alt;
+      reflexivity.
+Qed.
+
+(*
+Lemma dub_neg_node_transform :
+    forall (P : ptree) (E : formula) (S : subst_ind),
+        struct_valid P ->
+            subst_ind_fit (ptree_formula P) S = true ->
+                { L : list subst_ind & node_extract (dub_neg_sub_ptree P E S) = (dub_neg_trans (combine (node_extract P) L) E) /\ length L = length (node_extract P) }.
+Proof.
+intros P.
+induction P;
+intros E S PSV FS;
+unfold dub_neg_sub_ptree, node_extract, dub_neg_sub_ptree_fit;
+rewrite FS;
+fold node_extract dub_neg_sub_ptree_fit.
+
+1 : destruct PSV. (*node*)
+2 : destruct PSV as [PSV DU]. (*deg up*)
+3 : destruct PSV as [[PSV OU] NO]. (*ord up*)
+
+4-13 : destruct PSV as [[[PF PSV] PD] PO]. (*single hyp*)
+14 : destruct PSV as [[[[PF PSV] PD] PO] CPF]. (*weakening*)
+
+15-19 : destruct PSV as [[[[[[[P1F P1SV] P1D] P1O] P2F] P2SV] P2D] P2O]. (*double hyp*)
+20-21 : destruct PSV as [[[[[[[[P1F P1SV] P1D] P1O] P2F] P2SV] P2D] P2O] INA]. (*loop*)
+
+1 : refine (existT _ [S] (conj eq_refl eq_refl)).
+
+
+3-6,8-15,18-20 :
+  destruct S;
+  inversion FS as [FS'];
+  try rewrite FS';
+  try destruct (and_bool_prop _ _ FS') as [FS1 FS2].
+
+4-6,10,13,17 :
+  destruct S1;
+  inversion FS' as [FS''];
+  try rewrite FS'';
+  try destruct (and_bool_prop _ _ FS1) as [FS1_1 FS1_2].
+
+6 : destruct S1_1;
+  inversion FS'' as [FS'''];
+  try rewrite FS''';
+  destruct (and_bool_prop _ _ FS1_1) as [FS1_1_1 FS1_1_2].
+
+8,15 : case form_eqb eqn:EQ.
+
+all : repeat rewrite dub_neg_ptree_formula_true;
+      unfold node_extract, ptree_formula in *;
+      fold node_extract ptree_formula in *;
+      try apply (IHP _ _ PSV);
+      repeat rewrite app_length;
+      try destruct (IHP1 E _ P1SV) as [L1 EQ1];
+      try destruct (IHP2 _ _ P2SV) as [L2 EQ2];
+      try rewrite PF;
+      try rewrite P1F;
+      try rewrite P2F;
+      unfold subst_ind_fit;
+      fold subst_ind_fit;
+      try rewrite FS;
+      try rewrite FS';
+      try rewrite FS1;
+      try rewrite FS2;
+      try rewrite FS1_1;
+      try rewrite FS1_2;
+      try rewrite FS1_1_1;
+      try rewrite FS1_1_2;
+      try rewrite non_target_fit;
+      try rewrite non_target_sub_fit;
+      try reflexivity.
+
+  15 :  try refine (existT _ ((map non_target (node_extract P1)) ++ (projT1 (IHP2 E _ P2SV _))) (conj _ _));
+        try destruct IHP2 as [L2 [EQ2 EL2]];
+        unfold projT1, dub_neg_trans;
+        try rewrite <- (combine_eq_len _ _ _ _ (eq_sym (map_length _ _)));
+        try rewrite map_app;
+        try rewrite app_length;
+        try rewrite map_length;
+        try rewrite EL2;
+        try rewrite (combine_non_target_triv (node_extract P1) E) at 1;
+        try rewrite EQ2;
+        try reflexivity.
+
+  14 :  try refine (existT _ ((projT1 (IHP1 E _ P1SV _)) ++ (map non_target (node_extract P2))) (conj _ _));
+        try destruct IHP1 as [L1 [EQ1 EL1]];
+        unfold projT1, dub_neg_trans;
+        try rewrite <- (combine_eq_len _ _ _ _ (eq_sym EL1));
+        try rewrite map_app;
+        try rewrite app_length;
+        try rewrite map_length;
+        try rewrite EL1;
+        try rewrite (combine_non_target_triv (node_extract P2) E) at 1;
+        try rewrite EQ1;
+        try reflexivity.
+
+  1,2,5-7 : refine (existT _ (map non_target (node_extract P)) (conj _ _));
+            unfold dub_neg_trans;
+            try rewrite (combine_non_target_triv (node_extract P) E) at 1;
+            repeat rewrite map_length;
+            reflexivity.
+  
+  1,2,5 : try refine (existT _ ((projT1 (IHP1 E _ P1SV _)) ++ (projT1 (IHP2 E _ P2SV _))) (conj _ _));
+          try destruct IHP1 as [L1 [EQ1 EL1]], IHP2 as [L2 [EQ2 EL2]];
+          unfold projT1;
+          try rewrite <- (combine_eq_len _ _ _ _ (eq_sym EL1));
+          try rewrite EQ1,EQ2;
+          unfold dub_neg_trans;
+          try rewrite map_app;
+          try rewrite app_length, EL1, EL2;
+          try reflexivity.
+
+  1,2 : refine (existT _ (map non_target ((node_extract P1) ++ (node_extract P2))) (conj _ _));
+        unfold dub_neg_trans;
+        rewrite map_app;
+        try rewrite <- (combine_eq_len _ _ _ _ (eq_sym (map_length _ _)));
+        try rewrite map_app;
+        try rewrite (combine_non_target_triv (node_extract P1) E) at 1;
+        try rewrite (combine_non_target_triv (node_extract P2) E) at 1;
+        try rewrite app_length;
+        repeat rewrite map_length;
+        try reflexivity.
+
+  1,2 : refine (existT _ (map non_target ((remove form_eq_dec a (node_extract P2)) ++ (node_extract P1))) (conj _ _));
+        unfold dub_neg_trans;
+        rewrite map_app;
+        try rewrite <- (combine_eq_len _ _ _ _ (eq_sym (map_length _ _)));
+        try rewrite map_app;
+        try rewrite (combine_non_target_triv (node_extract P1) E) at 1;
+        try rewrite (combine_non_target_triv (remove form_eq_dec a (node_extract P2)) E) at 1;
+        try rewrite app_length;
+        repeat rewrite map_length;
+        try reflexivity.
+
+  1 : { assert (subst_ind_fit (ptree_formula P2) (lor_ind S1 (non_target a)) = true) as FSC.
+        { rewrite P2F.
+          unfold subst_ind_fit;
+          fold subst_ind_fit.
+          rewrite FS1.
+          apply non_target_sub_fit. }
+        try refine (existT _ ((snd (split (filter (fun X : (formula * subst_ind) => (if form_eq_dec (lor c a) (fst X) then false else true)) (combine (node_extract P2) (projT1 (IHP2 E _ P2SV FSC)))))) ++ (projT1 (IHP1 E _ P1SV _))) (conj _ _));
+        try destruct IHP1 as [L1 [EQ1 EL1]], IHP2 as [L2 [EQ2 EL2]];
+        unfold projT1.
+        - unfold dub_neg_trans.
+          rewrite <- combine_eq_len.
+          + rewrite map_app, EQ1, EQ2.
+            refine (eq_app_eq _ _ _ _ _ (eq_refl)).
+            rewrite <- (remove_alt _ (lor c a)).
+            unfold remove'.
+            rewrite (combine_with_filter_split (fun Y => if form_eq_dec (lor c a) Y then false else true) (node_extract P2) L2 (eq_sym EL2)).
+
+            admit.
+          + admit.
+
+        - rewrite app_length, split_length_r, EL1.
+          rewrite (combine_filter_fst _ _ (fun X => (if form_eq_dec (lor c a) X then false else true)) (eq_sym EL2)).
+          rewrite <- remove_alt.
+          unfold remove'.
+          reflexivity. }
+
+
+
+Admitted.
+*)
+
+Lemma dub_neg_node_len : 
+    forall (P : ptree) (S : subst_ind),
+        struct_valid P ->
+            length (node_extract P) = length (dub_neg_node P S).
+Proof.
+intros P;
+induction P;
+intros S PSV;
+unfold dub_neg_node;
+case subst_ind_fit eqn:FS;
+try rewrite map_length;
+try reflexivity;
+unfold node_extract, dub_neg_node_fit;
+fold node_extract dub_neg_node_fit.
+
+1 : destruct PSV as [PSV DU]. (*deg up*)
+2 : destruct PSV as [[PSV OU] NO]. (*ord up*)
+
+3-12 : destruct PSV as [[[PF PSV] PD] PO]. (*single hyp*)
+13 : destruct PSV as [[[[PF PSV] PD] PO] CPF]. (*weakening*)
+
+14-18 : destruct PSV as [[[[[[[P1F P1SV] P1D] P1O] P2F] P2SV] P2D] P2O]. (*double hyp*)
+19-20 : destruct PSV as [[[[[[[[P1F P1SV] P1D] P1O] P2F] P2SV] P2D] P2O] INA]. (*loop*)
+
+all : unfold ptree_formula in *;
+      fold ptree_formula in *.
+
+3-6,8-15,18-20 :
+  destruct S;
+  inversion FS as [FS'];
+  try rewrite FS';
+  try destruct (and_bool_prop _ _ FS') as [FS1 FS2].
+
+4-6,10,13,17 :
+  destruct S1;
+  inversion FS' as [FS''];
+  try rewrite FS'';
+  try destruct (and_bool_prop _ _ FS1) as [FS1_1 FS1_2].
+
+6 : destruct S1_1;
+  inversion FS'' as [FS'''];
+  try rewrite FS''';
+  destruct (and_bool_prop _ _ FS1_1) as [FS1_1_1 FS1_1_2].
+
+all : repeat rewrite dub_neg_node_formula_true;
+      try apply IHP;
+      repeat rewrite app_length;
+      try rewrite <- IHP1;
+      try rewrite <- IHP2;
+      try apply PSV;
+      try apply P1SV;
+      try apply P2SV;
+      try apply FS;
+      try rewrite PF;
+      try rewrite P1F;
+      try rewrite P2F;
+      unfold subst_ind_fit;
+      fold subst_ind_fit;
+      repeat rewrite FS;
+      try rewrite FS1;
+      try rewrite FS2;
+      try rewrite FS1_1;
+      try rewrite FS1_2;
+      try rewrite FS1_1_1;
+      try rewrite FS1_1_2;
+      try rewrite non_target_fit;
+      try rewrite non_target_sub_fit;
+      try reflexivity.
+
+all : rewrite split_length_r, <- remove_alt;
+      unfold remove';
+      rewrite (combine_filter_fst _ _ (fun X => if (form_eq_dec _ X) then false else true));
+      try reflexivity;
+      apply IHP2, P2SV.
+Qed.
+
+(*
+Lemma dub_neg_non_target_triv_len :
+    forall (LF : list formula) (P : ptree),
+        LF = node_extract P ->
+            forall (E : formula),
+                struct_valid P ->
+                    node_extract P = dub_neg_trans (combine (node_extract P) (dub_neg_node P (non_target (ptree_formula P)))) E.
+Proof.
+intros LF.
+induction LF as [LF IND] using (induction_ltof1 _ (@length formula)).
+
+induction P;
+intros EQL E PSV;
+unfold dub_neg_trans, dub_neg_node, dub_neg_node_fit, ptree_formula, node_extract;
+rewrite non_target_fit;
+fold ptree_formula node_extract dub_neg_node_fit.
+
+1 : destruct PSV. (*node*)
+2 : destruct PSV as [PSV DU]. (*deg up*)
+3 : destruct PSV as [[PSV OU] NO]. (*ord up*)
+
+4-13 : destruct PSV as [[[PF PSV] PD] PO]. (*single hyp*)
+14 : destruct PSV as [[[[PF PSV] PD] PO] CPF]. (*weakening*)
+
+15-19 : destruct PSV as [[[[[[[P1F P1SV] P1D] P1O] P2F] P2SV] P2D] P2O]. (*double hyp*)
+20-21 : destruct PSV as [[[[[[[[P1F P1SV] P1D] P1O] P2F] P2SV] P2D] P2O] INA]. (*loop*)
+
+1 : unfold combine, map, fst, snd, dub_neg_sub_formula.
+    rewrite non_target_sub.
+    reflexivity.
+
+all : unfold non_target;
+      fold non_target;
+      unfold node_extract in EQL;
+      fold node_extract in EQL;
+      repeat rewrite dub_neg_node_formula_true;
+      try rewrite PF;
+      try rewrite P1F;
+      try rewrite P2F;
+      try apply non_target_fit;
+      unfold subst_ind_fit;
+      fold subst_ind_fit;
+      try rewrite non_target_fit;
+      try apply non_target_sub_fit;
+      repeat rewrite non_target_lor;
+      try rewrite <- PF;
+      try rewrite <- P1F;
+      try rewrite <- P2F.
+
+11,12 : fold (non_target (neg (substitution a m (projT1 t))));
+        try rewrite non_target_lor;
+        rewrite <- PF.
+
+all : try apply (IHP EQL _ PSV).
+
+1-5 : try rewrite <- (combine_eq_len _ _ _ _ (dub_neg_node_len _ _ P1SV));
+      try rewrite map_app;
+      unfold ltof in IND;
+      rewrite EQL in IND;
+      rewrite (IND _ (struct_node_sum_less_l) _ eq_refl E P1SV), (IND _ (struct_node_sum_less_r) _ eq_refl E P2SV) at 1;
+      rewrite P1F, P2F;
+      reflexivity.
+
+1 : { rewrite <- remove_alt at 2.
+      unfold remove'.
+      rewrite <- combine_eq_len.
+      rewrite (combine_with_filter_split (fun Y => if form_eq_dec a Y then false else true) (node_extract P2)).
+      - rewrite map_app.
+        destruct (remove form_eq_dec a (node_extract P2)) as [ | L2] eqn:EQ.
+        + rewrite app_nil_l in *.
+          rewrite (IHP1 EQL E P1SV) at 1.
+          admit.
+        + unfold ltof in IND;
+        rewrite EQL in IND;
+        rewrite (IND _ (struct_node_sum_less_l) _ EQ E P2SV), (IND _ (struct_node_sum_less_r) _ eq_refl E P2SV) at 1;
+        rewrite P1F, P2F;
+        reflexivity.
+
+      - apply dub_neg_node_len, P2SV.
+      - rewrite split_length_r.
+        rewrite <- (combine_filter_fst _ (dub_neg_node P2 (non_target a))).
+        reflexivity.
+        apply dub_neg_node_len, P2SV. }
+
+1 : { rewrite <- remove_alt at 2.
+      unfold remove'.
+      rewrite <- combine_eq_len.
+      rewrite (combine_with_filter_split (fun Y => if form_eq_dec (lor c a) Y then false else true) (node_extract P2)).
+      - admit.
+      - apply dub_neg_node_len, P2SV.
+      - rewrite split_length_r.
+        rewrite <- (combine_filter_fst _ (dub_neg_node P2 (non_target (lor c a)))).
+        reflexivity.
+        apply dub_neg_node_len, P2SV. }
+
+
+Qed.
+*)
+
+Lemma dub_neg_non_target_triv :
+    forall (P : ptree) (E : formula),
+        struct_valid P ->
+            node_extract P = dub_neg_trans (combine (node_extract P) (dub_neg_node P (non_target (ptree_formula P)))) E.
+Proof.
+intros P;
+induction P;
+intros E PSV;
+unfold dub_neg_trans, dub_neg_node, dub_neg_node_fit, ptree_formula, node_extract;
+rewrite non_target_fit;
+fold ptree_formula node_extract dub_neg_node_fit.
+
+1 : destruct PSV. (*node*)
+2 : destruct PSV as [PSV DU]. (*deg up*)
+3 : destruct PSV as [[PSV OU] NO]. (*ord up*)
+
+4-13 : destruct PSV as [[[PF PSV] PD] PO]. (*single hyp*)
+14 : destruct PSV as [[[[PF PSV] PD] PO] CPF]. (*weakening*)
+
+15-19 : destruct PSV as [[[[[[[P1F P1SV] P1D] P1O] P2F] P2SV] P2D] P2O]. (*double hyp*)
+20-21 : destruct PSV as [[[[[[[[P1F P1SV] P1D] P1O] P2F] P2SV] P2D] P2O] INA]. (*loop*)
+
+1 : unfold combine, map, fst, snd, dub_neg_sub_formula.
+    rewrite non_target_sub.
+    reflexivity.
+
+all : unfold non_target;
+      fold non_target;
+      repeat rewrite dub_neg_node_formula_true;
+      try rewrite PF;
+      try rewrite P1F;
+      try rewrite P2F;
+      try apply non_target_fit;
+      unfold subst_ind_fit;
+      fold subst_ind_fit;
+      try rewrite non_target_fit;
+      try apply non_target_sub_fit;
+      repeat rewrite non_target_lor;
+      try rewrite <- PF;
+      try rewrite <- P1F;
+      try rewrite <- P2F.
+
+11,12 :  fold (non_target (neg (substitution a m (projT1 t))));
+      try rewrite non_target_lor;
+      rewrite <- PF.
+
+all : try apply (IHP _ PSV).
+
+1-5 : try rewrite <- (combine_eq_len _ _ _ _ (dub_neg_node_len _ _ P1SV));
+      try rewrite map_app;
+      try rewrite (IHP1 E P1SV) at 1;
+      try rewrite (IHP2 E P2SV) at 1;
+      try rewrite P1F, P2F;
+      try reflexivity.
+      
+1 : { rewrite <- remove_alt at 2.
+      unfold remove'.
+      rewrite <- combine_eq_len.
+      rewrite (combine_with_filter_split (fun Y => if form_eq_dec a Y then false else true) (node_extract P2)).
+      - rewrite map_app.
+        fold (dub_neg_trans (combine (node_extract P1) (dub_neg_node P1 (non_target a))) E).
+        rewrite (non_target_term_sub a n zero) at 2.
+        rewrite <- P1F.
+        rewrite <- (IHP1 _ P1SV).
+        admit.
+
+      - apply dub_neg_node_len, P2SV.
+      - rewrite split_length_r.
+        rewrite <- (combine_filter_fst _ (dub_neg_node P2 (non_target a))).
+        reflexivity.
+        apply dub_neg_node_len, P2SV. }
+
+1 : { rewrite <- remove_alt at 2.
+      unfold remove'.
+      rewrite <- combine_eq_len.
+      rewrite (combine_with_filter_split (fun Y => if form_eq_dec (lor c a) Y then false else true) (node_extract P2)).
+      - admit.
+      - apply dub_neg_node_len, P2SV.
+      - rewrite split_length_r.
+        rewrite <- (combine_filter_fst _ (dub_neg_node P2 (non_target (lor c a)))).
+        reflexivity.
+        apply dub_neg_node_len, P2SV. }
+Admitted.
+
+Lemma dub_neg_node_transform_other :
+    forall (P : ptree) (E : formula) (S : subst_ind),
+        struct_valid P ->
+            subst_ind_fit (ptree_formula P) S = true ->
+                node_extract (dub_neg_sub_ptree P E S) = (dub_neg_trans (combine (node_extract P) (dub_neg_node P S)) E).
+Proof.
+intros P.
+induction P;
+intros E S PSV FS;
+unfold dub_neg_sub_ptree, node_extract, dub_neg_sub_ptree_fit, dub_neg_node, dub_neg_node_fit;
+rewrite FS;
+fold node_extract dub_neg_sub_ptree_fit dub_neg_node_fit.
+
+1 : destruct PSV. (*node*)
+2 : destruct PSV as [PSV DU]. (*deg up*)
+3 : destruct PSV as [[PSV OU] NO]. (*ord up*)
+
+4-13 : destruct PSV as [[[PF PSV] PD] PO]. (*single hyp*)
+14 : destruct PSV as [[[[PF PSV] PD] PO] CPF]. (*weakening*)
+
+15-19 : destruct PSV as [[[[[[[P1F P1SV] P1D] P1O] P2F] P2SV] P2D] P2O]. (*double hyp*)
+20-21 : destruct PSV as [[[[[[[[P1F P1SV] P1D] P1O] P2F] P2SV] P2D] P2O] INA]. (*loop*)
+
+1 : reflexivity.
+
+3-6,8-15,18-20 :
+  destruct S;
+  inversion FS as [FS'];
+  try rewrite FS';
+  try destruct (and_bool_prop _ _ FS') as [FS1 FS2].
+
+4-6,10,13,17 :
+  destruct S1;
+  inversion FS' as [FS''];
+  try rewrite FS'';
+  try destruct (and_bool_prop _ _ FS1) as [FS1_1 FS1_2].
+
+6 : destruct S1_1;
+  inversion FS'' as [FS'''];
+  try rewrite FS''';
+  destruct (and_bool_prop _ _ FS1_1) as [FS1_1_1 FS1_1_2].
+
+8,15 : case form_eqb eqn:EQ.
+
+all : repeat rewrite dub_neg_ptree_formula_true;
+      repeat rewrite dub_neg_node_formula_true;
+      unfold node_extract, ptree_formula in *;
+      fold node_extract ptree_formula in *;
+      try rewrite (IHP _ _ PSV);
+      try rewrite (IHP1 _ _ P1SV);
+      try rewrite (IHP2 _ _ P2SV); 
+      try rewrite PF;
+      try rewrite P1F;
+      try rewrite P2F;
+      unfold subst_ind_fit;
+      fold subst_ind_fit;
+      try rewrite FS;
+      try rewrite FS';
+      try rewrite FS1;
+      try rewrite FS2;
+      try rewrite FS1_1;
+      try rewrite FS1_2;
+      try rewrite FS1_1_1;
+      try rewrite FS1_1_2;
+      try rewrite non_target_fit;
+      try rewrite non_target_sub_fit;
+      try reflexivity.
+
+  15 :  try refine (existT _ ((map non_target (node_extract P1)) ++ (projT1 (IHP2 E _ P2SV _))) (conj _ _));
+        try destruct IHP2 as [L2 [EQ2 EL2]];
+        unfold projT1, dub_neg_trans;
+        try rewrite <- (combine_eq_len _ _ _ _ (eq_sym (map_length _ _)));
+        try rewrite map_app;
+        try rewrite app_length;
+        try rewrite map_length;
+        try rewrite EL2;
+        try rewrite (combine_non_target_triv (node_extract P1) E) at 1;
+        try rewrite EQ2;
+        try reflexivity.
+
+  14 :  try refine (existT _ ((projT1 (IHP1 E _ P1SV _)) ++ (map non_target (node_extract P2))) (conj _ _));
+        try destruct IHP1 as [L1 [EQ1 EL1]];
+        unfold projT1, dub_neg_trans;
+        try rewrite <- (combine_eq_len _ _ _ _ (eq_sym EL1));
+        try rewrite map_app;
+        try rewrite app_length;
+        try rewrite map_length;
+        try rewrite EL1;
+        try rewrite (combine_non_target_triv (node_extract P2) E) at 1;
+        try rewrite EQ1;
+        try reflexivity.
+
+  1,2,5-7 : unfold 
+  refine (existT _ (map non_target (node_extract P)) (conj _ _));
+            unfold dub_neg_trans;
+            try rewrite (combine_non_target_triv (node_extract P) E) at 1;
+            repeat rewrite map_length;
+            reflexivity.
+  
+  1,2,5 : try refine (existT _ ((projT1 (IHP1 E _ P1SV _)) ++ (projT1 (IHP2 E _ P2SV _))) (conj _ _));
+          try destruct IHP1 as [L1 [EQ1 EL1]], IHP2 as [L2 [EQ2 EL2]];
+          unfold projT1;
+          try rewrite <- (combine_eq_len _ _ _ _ (eq_sym EL1));
+          try rewrite EQ1,EQ2;
+          unfold dub_neg_trans;
+          try rewrite map_app;
+          try rewrite app_length, EL1, EL2;
+          try reflexivity.
+
+  1,2 : refine (existT _ (map non_target ((node_extract P1) ++ (node_extract P2))) (conj _ _));
+        unfold dub_neg_trans;
+        rewrite map_app;
+        try rewrite <- (combine_eq_len _ _ _ _ (eq_sym (map_length _ _)));
+        try rewrite map_app;
+        try rewrite (combine_non_target_triv (node_extract P1) E) at 1;
+        try rewrite (combine_non_target_triv (node_extract P2) E) at 1;
+        try rewrite app_length;
+        repeat rewrite map_length;
+        try reflexivity.
+
+  1,2 : refine (existT _ (map non_target ((remove form_eq_dec a (node_extract P2)) ++ (node_extract P1))) (conj _ _));
+        unfold dub_neg_trans;
+        rewrite map_app;
+        try rewrite <- (combine_eq_len _ _ _ _ (eq_sym (map_length _ _)));
+        try rewrite map_app;
+        try rewrite (combine_non_target_triv (node_extract P1) E) at 1;
+        try rewrite (combine_non_target_triv (remove form_eq_dec a (node_extract P2)) E) at 1;
+        try rewrite app_length;
+        repeat rewrite map_length;
+        try reflexivity.
+
+  1 : { assert (subst_ind_fit (ptree_formula P2) (lor_ind S1 (non_target a)) = true) as FSC.
+        { rewrite P2F.
+          unfold subst_ind_fit;
+          fold subst_ind_fit.
+          rewrite FS1.
+          apply non_target_sub_fit. }
+        try refine (existT _ ((snd (split (filter (fun X : (formula * subst_ind) => (if form_eq_dec (lor c a) (fst X) then false else true)) (combine (node_extract P2) (projT1 (IHP2 E _ P2SV FSC)))))) ++ (projT1 (IHP1 E _ P1SV _))) (conj _ _));
+        try destruct IHP1 as [L1 [EQ1 EL1]], IHP2 as [L2 [EQ2 EL2]];
+        unfold projT1.
+        - unfold dub_neg_trans.
+          rewrite <- combine_eq_len.
+          + rewrite map_app, EQ1, EQ2.
+            refine (eq_app_eq _ _ _ _ _ (eq_refl)).
+            rewrite <- (remove_alt _ (lor c a)).
+            unfold remove'.
+            rewrite (combine_with_filter_split (fun Y => if form_eq_dec (lor c a) Y then false else true) (node_extract P2) L2 (eq_sym EL2)).
+
+            admit.
+          + admit.
+
+        - rewrite app_length, split_length_r, EL1.
+          rewrite (combine_filter_fst _ _ (fun X => (if form_eq_dec (lor c a) X then false else true)) (eq_sym EL2)).
+          rewrite <- remove_alt.
+          unfold remove'.
+          reflexivity. }
+
+
+
+Admitted.
+
+
+(*
+Lemma dub_neg_node_size :
+    forall (P : ptree) (E : formula) (S : subst_ind),
+        struct_valid P ->
+            subst_ind_fit (ptree_formula P) S = true ->
+                length (node_extract P) = length (node_extract (dub_neg_sub_ptree P E S)).
+Proof.
+intros P.
+induction P;
+intros E S PSV FS;
+unfold dub_neg_sub_ptree, node_extract, dub_neg_sub_ptree_fit;
+rewrite FS;
+fold node_extract dub_neg_sub_ptree_fit.
+
+1 : destruct PSV. (*node*)
+2 : destruct PSV as [PSV DU]. (*deg up*)
+3 : destruct PSV as [[PSV OU] NO]. (*ord up*)
+
+4-13 : destruct PSV as [[[PF PSV] PD] PO]. (*single hyp*)
+14 : destruct PSV as [[[[PF PSV] PD] PO] CPF]. (*weakening*)
+
+15-19 : destruct PSV as [[[[[[[P1F P1SV] P1D] P1O] P2F] P2SV] P2D] P2O]. (*double hyp*)
+20-21 : destruct PSV as [[[[[[[[P1F P1SV] P1D] P1O] P2F] P2SV] P2D] P2O] INA]. (*loop*)
+
+1 : reflexivity.
+
+3-6,8-15,18-20 :
+      destruct S;
+      inversion FS as [FS'];
+      try rewrite FS';
+      try destruct (and_bool_prop _ _ FS') as [FS1 FS2].
+  
+4-6,10,13,17 :
+    destruct S1;
+    inversion FS' as [FS''];
+    try rewrite FS'';
+    try destruct (and_bool_prop _ _ FS1) as [FS1_1 FS1_2].
+  
+6 : destruct S1_1;
+    inversion FS'' as [FS'''];
+    try rewrite FS''';
+    destruct (and_bool_prop _ _ FS1_1) as [FS1_1_1 FS1_1_2].
+
+8,15 : case form_eqb eqn:EQ.
+
+all : repeat rewrite dub_neg_ptree_formula_true;
+      unfold node_extract, ptree_formula in *;
+      fold node_extract ptree_formula in *;
+      try apply (IHP _ _ PSV);
+      repeat rewrite app_length;
+      try rewrite <- (IHP1 _ _ P1SV);
+      try rewrite <- (IHP2 _ _ P2SV);
+      try rewrite PF;
+      try rewrite P1F;
+      try rewrite P2F;
+      unfold subst_ind_fit;
+      fold subst_ind_fit;
+      try rewrite FS;
+      try rewrite FS';
+      try rewrite FS1;
+      try rewrite FS2;
+      try rewrite FS1_1;
+      try rewrite FS1_2;
+      try rewrite FS1_1_1;
+      try rewrite FS1_1_2;
+      try rewrite non_target_fit;
+      try rewrite non_target_sub_fit;
+      try reflexivity.
+
+      rewrite remove_length.
+
+      admit.
+
+
+Lemma dub_neg_free_sub_aux :
+    forall (P : ptree) (E : formula) (S : subst_ind),
+        struct_valid P ->
+            subst_ind_fit (ptree_formula P) S = true ->
+                forall (A : formula),
+                    In A (node_extract (dub_neg_sub_ptree P E S)) ->
+                        { B : formula & In B (node_extract P) /\ free_list B = free_list A }.
+Proof.
+  intros P E.
+  induction P;
+  intros S PSV FS C INC.
+
+  1 : destruct PSV. (*node*)
+  2 : destruct PSV as [PSV DU]. (*deg up*)
+  3 : destruct PSV as [[PSV OU] NO]. (*ord up*)
+
+  4-13 : destruct PSV as [[[PF PSV] PD] PO]. (*single hyp*)
+  14 : destruct PSV as [[[[PF PSV] PD] PO] CPF]. (*weakening*)
+
+  15-19 : destruct PSV as [[[[[[[P1F P1SV] P1D] P1O] P2F] P2SV] P2D] P2O]. (*double hyp*)
+  20-21 : destruct PSV as [[[[[[[[P1F P1SV] P1D] P1O] P2F] P2SV] P2D] P2O] INA]. (*loop*)
+  
+  1 : { exists a.
+        repeat split.
+        apply or_introl, eq_refl.
+        unfold dub_neg_sub_ptree, node_extract, dub_neg_sub_ptree_fit in INC.
+        rewrite FS in INC.
+        inversion INC as [EQ | FAL].
+        destruct EQ.
+        rewrite dub_neg_formula_free.
+        reflexivity.
+        inversion FAL. }
+  
+  3-6,8-15,18-20 :
+      destruct S;
+      inversion FS as [FS'];
+      try rewrite FS';
+      try destruct (and_bool_prop _ _ FS') as [FS1 FS2].
+  
+  4-6,10,13,17 :
+      destruct S1;
+      inversion FS' as [FS''];
+      try rewrite FS'';
+      try destruct (and_bool_prop _ _ FS1) as [FS1_1 FS1_2].
+  
+  6 : destruct S1_1;
+      inversion FS'' as [FS'''];
+      try rewrite FS''';
+      destruct (and_bool_prop _ _ FS1_1) as [FS1_1_1 FS1_1_2].
+  
+  all : unfold dub_neg_sub_ptree in INC;
+        rewrite FS in INC;
+        unfold dub_neg_sub_ptree_fit in INC;
+        fold dub_neg_sub_ptree_fit in INC;
+        unfold node_extract in *;
+        fold node_extract in *;
+        try rewrite dub_neg_ptree_formula_true in INC;
+        try rewrite dub_neg_ptree_formula_true in INC;
+        try rewrite PF;
+        try rewrite P1F;
+        try rewrite P2F;
+        unfold ptree_formula in FS;
+        fold ptree_formula in FS;
+        unfold subst_ind_fit;
+        fold subst_ind_fit;
+        try rewrite FS;
+        try rewrite FS';
+        try rewrite FS1;
+        try rewrite FS2;
+        try rewrite FS1_1;
+        try rewrite FS1_2;
+        try rewrite FS1_1_1;
+        try rewrite FS1_1_2;
+        try rewrite non_target_fit;
+        try rewrite non_target_sub_fit;
+        try reflexivity.
+
+24 :  { try apply (@in_app_bor _ form_eq_dec) in INC as [INC1 | INC2].
+        - apply in_remove in INC1 as [INC1 NE].
+          destruct (fun FSUB => IHP2 _ P2SV FSUB C INC1) as [B [INB FB]].
+          + rewrite P2F.
+            unfold subst_ind_fit;
+            fold subst_ind_fit.
+            rewrite FS1.
+            apply non_target_sub_fit.
+          + 
+        - destruct (fun FSUB => IHP1 _ P1SV FSUB C INC2) as [B [INB FB]].
+          + rewrite P1F.
+            unfold subst_ind_fit;
+            fold subst_ind_fit.
+            rewrite FS1.
+            apply non_target_sub_fit.
+          + apply (existT _ B (conj (in_or_app _ _ _ (or_intror INB)) FB)).
+      }
+
+  all : try case form_eqb eqn:EQ;
+        unfold flat_map;
+        fold (flat_map free_list);
+        repeat rewrite flat_map_app;
+        repeat apply incl_app_app;
+        try apply incl_refl;
+        try apply (fun FSUB => IHP _ PSV FSUB _ INC);
+        try apply (existT _ C (conj INC eq_refl));
+        try apply (@in_app_bor _ form_eq_dec) in INC as [INC1 | INC2];
+        try apply (existT _ C (conj (in_or_app _ _ _ (or_introl INC1)) eq_refl));
+        try apply (existT _ C (conj (in_or_app _ _ _ (or_intror INC2)) eq_refl));
+        try destruct (fun FSUB => IHP1 _ P1SV FSUB C INC1) as [B [INB FB]];
+        try destruct (fun FSUB => IHP1 _ P1SV FSUB C INC2) as [B [INB FB]];
+        try destruct (fun FSUB => IHP2 _ P2SV FSUB C INC1) as [B [INB FB]];
+        try destruct (fun FSUB => IHP2 _ P2SV FSUB C INC2) as [B [INB FB]];
+        try apply (existT _ B (conj (in_or_app _ _ _ (or_introl INB)) FB));
+        try apply (existT _ B (conj (in_or_app _ _ _ (or_intror INB)) FB));
+        try rewrite PF;
+        try rewrite P1F;
+        try rewrite P2F;
+        unfold ptree_formula in FS;
+        fold ptree_formula in FS;
+        unfold subst_ind_fit;
+        fold subst_ind_fit;
+        try rewrite FS;
+        try rewrite FS';
+        try rewrite FS1;
+        try rewrite FS2;
+        try rewrite FS1_1;
+        try rewrite FS1_2;
+        try rewrite FS1_1_1;
+        try rewrite FS1_1_2;
+        try rewrite non_target_fit;
+        try rewrite non_target_sub_fit;
+        try reflexivity.
+Qed.
+
 Lemma dub_neg_free_sub :
     forall (P : ptree) (E : formula) (S : subst_ind),
         struct_valid P ->
@@ -471,6 +1520,24 @@ Proof.
         try rewrite non_target_fit;
         try rewrite non_target_sub_fit;
         try reflexivity.
+
+  24 :  { unfold flat_map;
+          fold (flat_map free_list).
+          repeat rewrite flat_map_app.
+          apply incl_app_app.
+          - refine (@flat_map_equiv _ _ form_eq_dec nat_eq_dec _ _ _ _ _ _ _ INA).
+            + rewrite <- (dub_neg_formula_free (lor c a) E (lor_ind S1 (non_target a))).
+              unfold dub_neg_sub_formula.
+              rewrite formula_sub_ind_lor.
+              rewrite non_target_sub.
+              reflexivity.
+              rewrite FS1.
+              apply non_target_fit.
+            + apply IHP2.
+          - apply (fun FSUB => IHP1 _ P1SV FSUB).
+          
+
+ }
 
   all : try case form_eqb eqn:EQ;
         try case (closed (univ n a)) eqn:CuA;
@@ -661,6 +1728,7 @@ Proof.
       apply (in_or_app _ _ _ (or_intror INB1)).
       apply BAX1. }
 Qed.
+*)
 
 Lemma dub_neg_all_ax_trans : 
     forall (P : ptree) (E : formula) (S : subst_ind),
